rollback

trunk/examples/programs/toy/InfeasibleCoreExamples.bpl
@@ -4,137 +4,134 @@
 // Author: heizmann@informatik.uni-freiburg.de
 // Date: 2015-01-31
 
-  var a,b : [int]bool;
-  var k,j : int;
-
 /*
  * (array!) loop invariant: a == b
  */
-procedure noMemleak() returns () 
-modifies a,b,k;
-{
-  b := a; // (= b a)
-  k := 0; // (= b a)
+procedure noMemleak() returns () {
+  var a,b : [int]bool;
+  var k,j : int;
+  b := a;
+  k := 0;
   while(*) {
-    assume (a[k] == false); // (and (= (select a k) false) (= b a))
-    a[k] := true; // (and (not (select b k)) (= a (store b k true)))
-    a[k] := false; // (and (= (select a k) false) (= b a))
-    k := k + 1; // (exists ((v_k_9 Int)) (and (not (select a v_k_9)) (= b a)))
+    assume (a[k] == false);
+    a[k] := true;
+    a[k] := false;
+    k := k + 1;
   }
   assert(a == b);
 }
 
 
 
-// /*
-//  * loop invariant: a[0] == 42
-//  */
-// procedure firstElementUntouched() returns () {
-//   var a : [int]int;
-//   var k : int;
-//   var x : int;
-//   a[0] := 42;
-//   assume k>=0;
-//   assume k<=0;
-//   while(*) {
-//     k := k + 1;
-//     havoc x;
-//     a[k] := x;
-//   }
-//   assert(a[0] == 42);
-// }
-// 
-// 
-// 
-// 
-// /*
-//  * (nonlinear!) loop invariant: x*tmp>0
-//  * live variable analysis needed
-//  */
-// procedure nonlinearInvariant() returns ()
-// {
-//   var x,y: int;
-//   var tmp: int;
-//   var k: int;
-//   
-//   assume (x * y > 0);
-//   tmp := y;
-//   while (*) {
-//     tmp := (if (tmp>=0) then tmp+1 else tmp-1);
-//     y := y + 1;
-//   }
-//   assert (x>=0 ==> tmp>=0);
-// }
-// 
-// 
-// /*
-//  * loop invariant: x == 0
-//  */
-// procedure slicing() returns () {
-//   var x,k : int;
-//   x := 0;
-//   k := 0;
-//   while(*) {
-//     k := k + 1;
-//   }
-//   assert(x == 0);
-// }
-// 
-// 
-// /*
-//  * loop invariant: k >= 0
-//  */
-// procedure sign() returns () {
-//   var k : int;
-//   assume k>=0;
-//   assume k<=0;
-//   while(*) {
-//     k := k + 1;
-//   }
-//   assert(k != -1);
-// }
-// 
-// 
-// /*
-//  * Live variable analysis needed!
-//  * loop invariant: x == 0
-//  */
-// procedure LandesVersicherungsAnstalt() returns () {
-//   var x,k : int;
-//   k := 0;
-//   x := k;
-//   while(*) {
-//     k := k + 1;
-//   }
-//   assert(x == 0);
-// }
-// 
-// 
-// 
-// 
-// /*
-//  * Why do we replace assignments that are not in the infeasible core by havoc
-//  * and not by skip?
-//  * Consider the following trace
-//  *     y := 0; x := y; y := y + 1; assert(x == 0);
-//  * Positions 0,1,3 constitute an infeasible core.
-//  * If we would drop position 2, we would obtain the state assertion
-//  * y==0&&x==y at nondeterministic if. As a consequence we would conlude
-//  * that the second assert statement holds.
-//  * 
-//  */
-// procedure replaceAssingmentByHavoc() returns () {
-//   var x,y : int;
-//   y := 0;
-//   x := y;
-//   y := y + 1;
-//   if (*) {
-//     assert(x == 0);
-//   } else {
-//     assert(y == 0);
-//   }
-// }
-// 
-// 
-// 
-// 
+/*
+ * loop invariant: a[0] == 42
+ */
+procedure firstElementUntouched() returns () {
+  var a : [int]int;
+  var k : int;
+  var x : int;
+  a[0] := 42;
+  assume k>=0;
+  assume k<=0;
+  while(*) {
+    k := k + 1;
+    havoc x;
+    a[k] := x;
+  }
+  assert(a[0] == 42);
+}
+
+
+
+
+/*
+ * (nonlinear!) loop invariant: x*tmp>0
+ * live variable analysis needed
+ */
+procedure nonlinearInvariant() returns ()
+{
+  var x,y: int;
+  var tmp: int;
+  var k: int;
+  
+  assume (x * y > 0);
+  tmp := y;
+  while (*) {
+    tmp := (if (tmp>=0) then tmp+1 else tmp-1);
+    y := y + 1;
+  }
+  assert (x>=0 ==> tmp>=0);
+}
+
+
+/*
+ * loop invariant: x == 0
+ */
+procedure slicing() returns () {
+  var x,k : int;
+  x := 0;
+  k := 0;
+  while(*) {
+    k := k + 1;
+  }
+  assert(x == 0);
+}
+
+
+/*
+ * loop invariant: k >= 0
+ */
+procedure sign() returns () {
+  var k : int;
+  assume k>=0;
+  assume k<=0;
+  while(*) {
+    k := k + 1;
+  }
+  assert(k != -1);
+}
+
+
+/*
+ * Live variable analysis needed!
+ * loop invariant: x == 0
+ */
+procedure LandesVersicherungsAnstalt() returns () {
+  var x,k : int;
+  k := 0;
+  x := k;
+  while(*) {
+    k := k + 1;
+  }
+  assert(x == 0);
+}
+
+
+
+
+/*
+ * Why do we replace assignments that are not in the infeasible core by havoc
+ * and not by skip?
+ * Consider the following trace
+ *     y := 0; x := y; y := y + 1; assert(x == 0);
+ * Positions 0,1,3 constitute an infeasible core.
+ * If we would drop position 2, we would obtain the state assertion
+ * y==0&&x==y at nondeterministic if. As a consequence we would conlude
+ * that the second assert statement holds.
+ * 
+ */
+procedure replaceAssingmentByHavoc() returns () {
+  var x,y : int;
+  y := 0;
+  x := y;
+  y := y + 1;
+  if (*) {
+    assert(x == 0);
+  } else {
+    assert(y == 0);
+  }
+}
+
+
+
+
